Proof of correctness for loops

src/arch/x64/X64.Leakage_i.fst
@@ -12,9 +12,42 @@ open FStar.Tactics
 let combine_reg_taints regs1 regs2 =
     fun x -> merge_taint (regs1 x) (regs2 x)
 
-let combine_taint_states (ts:taintState) (ts1:taintState) (ts2:taintState) =
+let combine_reg_taints_monotone regs1 regs2: Lemma
+(forall r. Public? ((combine_reg_taints regs1 regs2) r) ==> Public? (regs1 r) /\ Public? (regs2 r))
+= ()
+
+let taintstate_monotone ts ts' = ( forall r. Public? (ts'.regTaint r) ==> Public? (ts.regTaint r)) /\ (Public? (ts'.flagsTaint) ==> Public? (ts.flagsTaint))
+
+val taintstate_monotone_trans: (ts1:taintState) -> (ts2:taintState) -> (ts3:taintState) ->
+Lemma (taintstate_monotone ts1 ts2 /\ taintstate_monotone ts2 ts3 ==> taintstate_monotone ts1 ts3)
+let taintstate_monotone_trans ts1 ts2 ts3 = ()
+
+val isConstant_monotone: (ts1:taintState) -> (ts2:taintState) -> (code:tainted_code) -> (fuel:nat) -> (s1:traceState) -> (s2:traceState) -> Lemma
+(isConstantTimeGivenStates code fuel ts2 s1 s2 /\ taintstate_monotone ts1 ts2 ==> isConstantTimeGivenStates code fuel ts1 s1 s2)
+
+let isConstant_monotone ts1 ts2 code fuel s1 s2 = ()
+
+val isExplicit_monotone: (ts:taintState) -> (ts1:taintState) -> (ts2:taintState) -> (code:tainted_code) -> (fuel:nat) -> (s1:traceState) -> (s2:traceState) -> Lemma
+(isExplicitLeakageFreeGivenStates code fuel ts ts1 s1 s2 /\ taintstate_monotone ts1 ts2 ==> isExplicitLeakageFreeGivenStates code fuel ts ts2 s1 s2)
+
+let isExplicit_monotone ts ts1 ts2 code fuel s1 s2 = ()
+
+val isExplicit_monotone2: (ts:taintState) -> (ts1:taintState) -> (ts2:taintState) -> (code:tainted_code) -> (fuel:nat) -> (s1:traceState) -> (s2:traceState) -> Lemma
+(isExplicitLeakageFreeGivenStates code fuel ts2 ts s1 s2 /\ taintstate_monotone ts1 ts2 ==> isExplicitLeakageFreeGivenStates code fuel ts1 ts s1 s2)
+
+let isExplicit_monotone2 ts ts1 ts2 code fuel s1 s2 = ()
+
+
+val combine_taint_states: (ts1:taintState) -> (ts2:taintState) -> (ts:taintState{taintstate_monotone ts1 ts /\ taintstate_monotone ts2 ts})
+let combine_taint_states (ts1:taintState) (ts2:taintState) =
   TaintState (combine_reg_taints ts1.regTaint ts2.regTaint) (merge_taint ts1.flagsTaint ts2.flagsTaint)
-  
+
+val check_if_block_consumes_fixed_time: (block:tainted_codes) -> (fuel:nat) -> (ts:taintState) -> Tot (bool * taintState)
+(decreases %[fuel; block])
+val check_if_code_consumes_fixed_time: (code:tainted_code) -> (fuel:nat) -> (ts:taintState) -> Tot (bool * taintState) (decreases %[fuel; code; 1])
+val check_if_loop_consumes_fixed_time: (code:tainted_code{While? code}) -> (fuel:nat) -> (ts:taintState) -> Tot (bool * taintState) (decreases %[fuel; code; 0])
+
+
 let rec check_if_block_consumes_fixed_time (block:tainted_codes) (fuel:nat) (ts:taintState) : bool * taintState =
   match block with
   | [] -> true, ts
@@ -48,13 +81,13 @@ and check_if_code_consumes_fixed_time (code:tainted_code) (fuel:nat) (ts:taintSt
       let validIfFalse, tsIfFalse = check_if_code_consumes_fixed_time ifFalse fuel ts in
       if (not validIfFalse) then (false, ts)
       else
-      (true, combine_taint_states ts tsIfTrue tsIfFalse)
-     
-  | _ -> false, ts
+      (true, combine_taint_states tsIfTrue tsIfFalse)   
 
-
-(*
-and check_if_loop_consumes_fixed_time (pred:tainted_ocmp) (body:tainted_code) (ts:taintState) : bool * taintState =
+  | While cond body -> check_if_loop_consumes_fixed_time code fuel ts 
+  
+and check_if_loop_consumes_fixed_time c (fuel:nat) (ts:taintState) : bool * taintState =
+  if fuel = 0 then true, ts else
+  let While pred body = c in
   let cond_taint = pred.ot in
   let o1 = operand_taint (get_fst_ocmp pred.o) ts in
   let o2 = operand_taint (get_snd_ocmp pred.o) ts in
@@ -68,12 +101,11 @@ and check_if_loop_consumes_fixed_time (pred:tainted_ocmp) (body:tainted_code) (t
     let o2Public = operand_does_not_use_secrets (get_snd_ocmp pred.o) ts in
     if (not o2Public) then (false, ts)
     else
-    let fixedTime, next_ts = check_if_code_consumes_fixed_time body ts in
-    let combined_ts = combine_taint_states ts ts next_ts in
-    if (combined_ts = ts) then true, combined_ts
-    else check_if_loop_consumes_fixed_time pred body combined_ts
-*)
-  
+    let fixedTime, next_ts = check_if_code_consumes_fixed_time body (fuel - 1) ts in
+    if (not fixedTime) then (false, ts)
+    else
+    let combined_ts = combine_taint_states ts next_ts in
+    check_if_loop_consumes_fixed_time c (fuel - 1) combined_ts
 
 val lemma_equal_eval_isConstant_aux: (code1: tainted_code) -> (code2:tainted_code) -> (fuel:nat) -> (ts:taintState) -> (ts':taintState) -> (s1 : traceState) -> (s2:traceState) -> Lemma ((forall s. taint_eval_code code1 fuel s == taint_eval_code code2 fuel s) ==> 
   isConstantTimeGivenStates code1 fuel ts s1 s2 /\ isExplicitLeakageFreeGivenStates code1 fuel ts ts' s1 s2 ==> isConstantTimeGivenStates code2 fuel ts s1 s2 /\ isExplicitLeakageFreeGivenStates code2 fuel ts ts' s1 s2)
@@ -82,7 +114,8 @@ let lemma_equal_eval_isConstant_aux code1 code2 fuel ts ts' s1 s2 = ()
 
 val lemma_equal_eval_isConstant: (code1: tainted_code) -> (code2:tainted_code) -> (fuel:nat) -> (ts:taintState) -> (ts':taintState) -> Lemma ((forall s. taint_eval_code code1 s == taint_eval_code code2 s) ==> 
   isConstantTime code1 fuel ts /\ isLeakageFree code1 fuel ts ts' ==> isConstantTime code2 fuel ts /\ isLeakageFree code2 fuel ts ts')
-  
+
+#set-options "--z3rlimit 20"
 let lemma_equal_eval_isConstant code1 code2 fuel ts ts' = FStar.Classical.forall_intro_2 (lemma_equal_eval_isConstant_aux code1 code2 fuel ts ts')
 
 val monotone_ok_eval: (code:tainted_code) -> (fuel:nat) -> (s:traceState) -> Lemma
@@ -105,7 +138,15 @@ let rec monotone_ok_eval code fuel s = match code with
     let st, b = taint_eval_ocmp s ifCond in
     let st = {st with trace=BranchPredicate(b)::s.trace} in
     if b then monotone_ok_eval ifTrue fuel st else monotone_ok_eval ifFalse fuel st
-  | While _ _ -> admit()
+  | While cond body -> 
+    if fuel = 0 then ()
+    else
+    let st, b = taint_eval_ocmp s cond in
+    if not b then ()
+    else 
+    let st = {st with trace=BranchPredicate(b)::s.trace} in
+    monotone_ok_eval body (fuel-1) st;
+    ()
 
 and monotone_ok_eval_block block fuel s =
   match block with
@@ -116,19 +157,41 @@ and monotone_ok_eval_block block fuel s =
     monotone_ok_eval_block tl fuel (Some?.v s');
     monotone_ok_eval hd fuel s
 
+val lemma_loop_taintstate_monotone: (ts:taintState) -> (code:tainted_code{While? code}) -> (fuel:nat) -> Lemma 
+(requires True)
+(ensures (let _, ts' = check_if_loop_consumes_fixed_time code fuel ts in
+  taintstate_monotone ts ts'))
+(decreases %[fuel; code])
+
+#set-options "--z3rlimit 40"
+let rec lemma_loop_taintstate_monotone ts code fuel =
+  if fuel = 0 then ()
+  else
+  let While pred body = code in
+  let b, ts' = check_if_code_consumes_fixed_time body (fuel-1) ts in
+  let combined_ts = combine_taint_states ts ts' in
+  lemma_loop_taintstate_monotone combined_ts code (fuel-1)
+
 val lemma_code_explicit_leakage_free: (ts:taintState) -> (code:tainted_code) -> (fuel:nat) -> (s1:traceState) -> (s2:traceState) -> Lemma
  (requires True)
  (ensures (let b, ts' = check_if_code_consumes_fixed_time code fuel ts in
   (b2t b ==> isConstantTimeGivenStates code fuel ts s1 s2 /\ isExplicitLeakageFreeGivenStates code fuel ts ts' s1 s2)))
- (decreases %[code; 0])
+ (decreases %[fuel; code; 1])
 
 val lemma_block_explicit_leakage_free: (ts:taintState) -> (codes:tainted_codes) -> (fuel:nat) -> (s1:traceState) -> (s2:traceState) -> Lemma
  (requires True)
  (ensures (let b, ts' = check_if_block_consumes_fixed_time codes fuel ts in
   (b2t b ==> isConstantTimeGivenStates (Block codes) fuel ts s1 s2 /\ isExplicitLeakageFreeGivenStates (Block codes) fuel ts ts' s1 s2)))
- (decreases %[codes;1])
+ (decreases %[fuel; codes; 2])
 
-let rec lemma_code_explicit_leakage_free ts code fuel s1 s2 = match code with
+val lemma_loop_explicit_leakage_free: (ts:taintState) -> (code:tainted_code{While? code}) -> (fuel:nat) -> (s1:traceState) -> (s2:traceState) -> Lemma  
+ (requires True)
+ (ensures (let b, ts' = check_if_loop_consumes_fixed_time code fuel ts in
+  (b2t b ==> isConstantTimeGivenStates code fuel ts s1 s2 /\ isExplicitLeakageFreeGivenStates code fuel ts ts' s1 s2)))
+ (decreases %[fuel; code; 0])
+
+#set-options "--z3rlimit 100"
+ let rec lemma_code_explicit_leakage_free ts code fuel s1 s2 = match code with
   | Ins ins -> lemma_ins_leakage_free ts fuel ins
   | Block block -> lemma_block_explicit_leakage_free ts block fuel s1 s2
   | IfElse ifCond ifTrue ifFalse ->     
@@ -145,7 +208,7 @@ let rec lemma_code_explicit_leakage_free ts code fuel s1 s2 = match code with
     monotone_ok_eval ifFalse fuel st2;
     lemma_code_explicit_leakage_free ts ifFalse fuel st1 st2;
     ()
-  | _ -> ()
+  | While _ _ -> lemma_loop_explicit_leakage_free ts code fuel s1 s2
 
 and lemma_block_explicit_leakage_free ts block fuel s1 s2 = match block with
   | [] -> ()
@@ -162,6 +225,48 @@ and lemma_block_explicit_leakage_free ts block fuel s1 s2 = match block with
     monotone_ok_eval (Block tl) fuel s'1;
     monotone_ok_eval (Block tl) fuel s'2
 
+and lemma_loop_explicit_leakage_free ts code fuel s1 s2 =
+  if fuel = 0 then ()
+  else
+  let b_fin, ts_fin = check_if_code_consumes_fixed_time code fuel ts in
+  let r1 = taint_eval_code code fuel s1 in
+  let r2 = taint_eval_code code fuel s2 in
+  let While cond body = code in
+  let (st1, b1) = taint_eval_ocmp s1 cond in
+  let (st2, b2) = taint_eval_ocmp s2 cond in
+  assert (b2t b_fin ==> constTimeInvariant ts s1 s2 /\ st1.state.ok /\ st2.state.ok ==> b1 = b2);
+  assert (b2t b_fin ==> constTimeInvariant ts s1 s2 /\ st1.state.ok /\ st2.state.ok ==> constTimeInvariant ts st1 st2);
+  if not b1 || not b2 then
+  (
+  lemma_loop_taintstate_monotone ts code fuel;
+  ()
+  )
+  else
+  let st'1 = ({st1 with trace = BranchPredicate(true)::st1.trace}) in
+  let st'2 = ({st2 with trace = BranchPredicate(true)::st2.trace}) in
+  assert (b2t b_fin ==> constTimeInvariant ts s1 s2 /\ st'1.state.ok /\ st'2.state.ok ==> constTimeInvariant ts st'1 st'2);
+  let b', ts' = check_if_code_consumes_fixed_time body (fuel-1) ts in
+  lemma_code_explicit_leakage_free ts body (fuel-1) st'1 st'2;
+  monotone_ok_eval body (fuel-1) st'1;
+  monotone_ok_eval body (fuel-1) st'2;
+  let st1 = taint_eval_code body (fuel - 1) st'1 in
+  let st2 = taint_eval_code body (fuel - 1) st'2 in
+  assert (None? st1 ==> r1 == st1);
+  assert (None? st2 ==> r2 == st2);
+  if (None? st1 || None? st2) then ()
+  else
+  let st1 = Some?.v st1 in
+  let st2 = Some?.v st2 in
+  if not st1.state.ok || not st2.state.ok then ()
+  else
+  let combined_ts = combine_taint_states ts ts' in
+  let b_aux, ts_aux = check_if_loop_consumes_fixed_time code (fuel-1) combined_ts in
+  lemma_loop_explicit_leakage_free combined_ts code (fuel-1) st1 st2;
+  isConstant_monotone ts combined_ts code (fuel-1) st1 st2;
+  isExplicit_monotone2 ts_aux ts combined_ts code (fuel-1) st1 st2;
+  assert (b2t b_fin ==> constTimeInvariant ts s1 s2 /\ st1.state.ok /\ st2.state.ok ==> constTimeInvariant ts' st1 st2);
+  ()
+  
 val lemma_code_leakage_free: (ts:taintState) -> (code:tainted_code) -> (fuel:nat) -> Lemma
  (let b, ts' = check_if_code_consumes_fixed_time code fuel ts in
   (b2t b ==> isConstantTime code fuel ts /\ isLeakageFree code fuel ts ts'))
